Selection sort from first principle.

src/SelectionSort.v
@@ -6,6 +6,8 @@ From Equations Require Import Equations.
 Import ListNotations.
 Import Tick.Notations.
 
+(** * Pure functions *)
+
 (* Select and selsort as given by Software Foundations Chapter 3 *)
 Fixpoint select (x: nat) (l: list nat) : nat * list nat :=
   match l with
@@ -23,97 +25,60 @@ Fixpoint selection_sort (l : list nat) (n : nat) : list nat :=
   | x :: r, S n' => let (y, r') := select x r in y :: selection_sort r' n'
 end.
 
-Fixpoint selectD (x : nat) (l : list nat) (outD : listA nat) : Tick (T (listA nat)) :=
-  Tick.tick >>
-  match l with
-  | [] => match outD with
-        | NilA => Tick.ret (Thunk NilA)
-        | _ => bottom
-        end
-  | h :: t => if x <=? h then 
-            match outD with
-            | ConsA _ t' =>
-                let+ tD := thunkD (selectD x t) t' in
-                Tick.ret (Thunk (ConsA (Thunk h) tD))
-            | _ => bottom
-            end else
-            match outD with
-            | ConsA _ t' =>
-                let+ tD := thunkD (selectD h t) t' in
-                Tick.ret (Thunk (ConsA (Thunk h) tD))
-            | _ => bottom
-            end
-    end.
-           
-(* The entire list must be forced to select smallest element *)
-Definition selectD' (x : nat) (xs : list nat) (outD : listA nat) : Tick (T (listA nat)) :=
-  Tick.MkTick (1 + length xs) (exact xs).
-
-
-Lemma selectD_selectD'_leq : forall x xs outD,
-    Tick.cost (selectD x xs outD) <= Tick.cost (selectD' x xs outD).
-Proof.
-  intros x xs. revert x.
-  induction xs as [|y ys]; intros.
-  - destruct outD; cbn; lia.
-  - destruct outD; cbn; destruct (x <=? y); simpl; try lia.
-    + destruct x2; simpl; try lia.
-      specialize (IHys x x0). unfold selectD' in IHys.
-      simpl in IHys. lia.
-    + destruct x2; simpl; try lia.
-      specialize (IHys y x0). unfold selectD' in IHys.
-      simpl in IHys. lia.
-Qed.
-
-Lemma selectD_selectD'_eq : forall x xs outD,
-    let (_, out) := select x xs in
-    outD = exact out ->
-    selectD x xs outD = selectD' x xs outD.
-Proof.
-  intros x xs. revert x.
-  induction xs as [|y ys]; intros.
-  - destruct outD; cbn; [reflexivity|inversion 1].
-  - destruct outD; cbn; destruct (x <=? y) eqn:Hleq; simpl.
-    + destruct (select x ys); inversion 1.
-    + destruct (select y ys); inversion 1.
-    + unfold Tick.bind. destruct (select x ys) eqn:Hselect.
-      inversion 1; subst. unfold selectD'.
-      unfold exact, Exact_list in H.
-      simp exact_listA in H.
-      simpl. specialize (IHys x (Exact_list l)).
-      rewrite Hselect in IHys. specialize (IHys eq_refl).
-      rewrite IHys. simpl; f_equal. lia.
-    + unfold Tick.bind. destruct (select y ys) eqn:Hselect.
-      inversion 1; subst. unfold selectD'.
-      unfold exact, Exact_list in H.
-      simp exact_listA in H.
-      simpl. specialize (IHys y (Exact_list l)).
-      rewrite Hselect in IHys. specialize (IHys eq_refl).
-      rewrite IHys. simpl; f_equal. lia.
-Qed.
-
-(* The entire list is forced one selection at a time*)
-Fixpoint selection_sortD (xs : list nat) (outD : listA nat) : Tick (T (listA nat)) :=
-  Tick.tick >>
-  match xs, outD with
-  | [], _ => Tick.ret (Thunk NilA)
-  | x :: xs', ConsA zD zsD =>
-    let+ _ := thunkD (selection_sortD xs') zsD in
-    let+ xsD := selectD x xs' (exact xs) in
-    Tick.ret xsD (* We invariably force the entire input list *)
-  | _, _ => bottom
-  end.
-
-Lemma sort_produces_element (n : nat) (x : nat) (xs : list nat) :
-  selection_sort (x :: xs) (S n) = fst (select x xs) :: selection_sort (snd (select x xs)) n.
-Proof.
-  simpl. destruct (select x xs). simpl. reflexivity.
-Qed.
-
 Definition head_def {a} (xs : list a) (d : a) : a :=
   match xs with
   | [] => d
   | x :: _ => x
+  end.
+
+
+(** * Demand functions *)
+
+Inductive prodA (A B : Type) : Type :=
+  | pairA : T A -> T B -> prodA A B.
+
+Arguments pairA {A} {B}.
+
+Check thunkD.
+
+Definition prodD {A B C D} (f : T A -> T C) (g : T B -> T D)
+  (p : prodA A B) : prodA C D :=
+  match p with
+  | pairA a b => pairA (f a) (g b)
+  end.
+
+Fixpoint selectD (x : nat) (l : list nat) (outD : prodA nat (listA nat)) : Tick (T (listA nat)) :=
+  Tick.tick >>
+  match l with
+  | [] => Tick.ret (Thunk NilA) 
+  | h :: t => if x <=? h then
+              let+ ysD := selectD x t (prodD id tailX outD) in
+              Tick.ret (Thunk (ConsA (exact h) ysD))
+            else
+              let+ ysD := selectD h t (prodD id tailX outD) in
+              Tick.ret (Thunk (ConsA (exact h) ysD))
+    end.
+           
+Fixpoint selection_sortD (l : list nat) (n : nat) (outD : listA nat) :
+  Tick (T (listA nat)) :=
+  Tick.tick >>
+  match l, n with
+  | _, 0 => match outD with
+           | NilA => Tick.ret Undefined
+           | _ => bottom
+           end
+  | [], _ => match outD with
+           | NilA => Tick.ret (Thunk NilA)
+           | _ => bottom
+           end
+  | x :: r, S n' => match outD with
+           | ConsA yD ysD =>
+               let (y, r') := select x r in
+               let+ xsD := thunkD (selection_sortD r' n') ysD in
+               let+ resD := selectD x r (pairA (exact y) xsD) in
+               Tick.ret (Thunk (ConsA (Thunk x) resD))
+           | _ => bottom
+           end
   end.
 
 (* We force the empty list or the first element only *)
@@ -121,13 +86,140 @@ Definition headD {a} (xs : list a) (d : a) (outD : a) : Tick (T (listA a)) :=
   Tick.tick >>
   match xs with
   | [] => Tick.ret (Thunk NilA)
-  | x :: _ => Tick.ret (Thunk (ConsA (Thunk x) (Undefined)))
+  | x :: _ => Tick.ret (Thunk (ConsA (Thunk x) Undefined))
   end.
 
 Definition head_selection_sortD (xs : list nat) (outD : nat) : Tick (T (listA nat)) :=
-  let+ list_headD := headD (selection_sort xs (length xs)) 0 outD in
-  let+ xsD := thunkD (selection_sortD xs) list_headD in
+  let res := selection_sort xs (length xs) in
+  let+ list_headD := headD res 0 outD in
+  let+ xsD := thunkD (selection_sortD xs (length xs)) list_headD in
   Tick.ret xsD.
+
+
+(** * Alternative defs (specs) *)
+
+(* The entire list must be forced to select smallest element *)
+Definition selectD' (x : nat) (xs : list nat) (outD : listA nat) : Tick (T (listA nat)) :=
+  Tick.MkTick (1 + length xs) (exact xs).
+
+(* The entire list is forced one selection at a time*)
+Fixpoint selection_sortD' (xs : list nat) (outD : listA nat) :
+  Tick (T (listA nat)) :=
+  Tick.tick >>
+  match xs, outD with
+  | [], _ => Tick.ret (Thunk NilA)
+  | x :: xs', ConsA zD zsD =>
+    let+ _ := thunkD (selection_sortD' xs') zsD in
+    let+ xsD := selectD' x xs' (exact xs) in
+    Tick.ret xsD (* We invariably force the entire input list *)
+  | _, _ => bottom
+  end.
+
+Definition head_selection_sortD' (xs : list nat) (outD : nat) : Tick (T (listA nat)) :=
+  let+ list_headD := headD (selection_sort xs (length xs)) 0 outD in
+  let+ xsD := thunkD (selection_sortD' xs) list_headD in
+  Tick.ret xsD.
+
+(** * Theorem for pure functions *)
+
+Lemma sort_produces_element (n : nat) (x : nat) (xs : list nat) :
+  selection_sort (x :: xs) (S n) = fst (select x xs) :: selection_sort (snd (select x xs)) n.
+Proof.
+  simpl. destruct (select x xs). simpl. reflexivity.
+Qed.
+
+(** * Equivalence between demand functions and specs *)
+
+Lemma selectD_selectD'_leq : forall x xs yD ysD outD,
+    Tick.cost (selectD x xs (pairA yD ysD)) <= Tick.cost (selectD' x xs outD).
+Proof.
+  intros x xs. revert x.
+  induction xs as [|y ys]; intros; simpl; try lia.
+  destruct (x <=? y); simpl.
+  - specialize (IHys x (id yD) (tailX ysD) outD).
+    unfold selectD' in IHys. simpl in IHys. lia.
+  - specialize (IHys y (id yD) (tailX ysD) outD).
+    unfold selectD' in IHys. simpl in IHys. lia.
+Qed.
+
+Lemma selectD_selectD'_eq : forall x xs outD,
+    let (y, ys) := select x xs in
+    forall yD ysD,
+      yD `is_approx` y ->
+      ysD `is_approx` ys ->
+      outD = exact ys ->
+      selectD x xs (pairA yD ysD) = selectD' x xs outD.
+Proof.
+  intros x xs. revert x.
+  induction xs as [|x' xs']; intros.
+  - intros yD ysD Hly Hlys ->. reflexivity.
+  - simpl. destruct (x <=? x') eqn:Hleq; simpl.
+    + destruct (select x xs') eqn:Hselect.
+      intros yD ysD Hly Hlys ->.
+      unfold selectD', Tick.bind. simpl.
+      specialize (IHxs' x (exact l)).
+      rewrite Hselect in IHxs'.
+      inversion Hlys; subst.
+      * simpl. specialize (IHxs' yD Undefined Hly).
+        assert (Hundef: Undefined `less_defined` exact l) by solve_approx.
+        specialize (IHxs' Hundef eq_refl).
+        unfold selectD' in IHxs'. 
+        unfold id. rewrite IHxs'; simpl.
+        f_equal. lia.
+      * simpl. inversion H1; subst.
+        specialize (IHxs' yD xs Hly H4 eq_refl).
+        unfold id. rewrite IHxs'. unfold selectD'; simpl.
+        f_equal. lia.
+    + destruct (select x' xs') eqn:Hselect.
+      intros yD ysD Hly Hlys ->.
+      unfold selectD', Tick.bind. simpl.
+      specialize (IHxs' x' (exact l)).
+      rewrite Hselect in IHxs'.
+      inversion Hlys; subst.
+      * simpl. specialize (IHxs' yD Undefined Hly).
+        assert (Hundef: Undefined `less_defined` exact l) by solve_approx.
+        specialize (IHxs' Hundef eq_refl).
+        unfold selectD' in IHxs'. 
+        unfold id. rewrite IHxs'; simpl.
+        f_equal. lia.
+      * simpl. inversion H1; subst.
+        specialize (IHxs' yD xs Hly H4 eq_refl).
+        unfold id. rewrite IHxs'. unfold selectD'; simpl.
+        f_equal. lia.
+Qed.
+
+Lemma selection_sortD_sortD' (xs : list nat) (outD : listA nat) :
+  forall n, n >= length xs ->
+  Tick.cost (selection_sortD xs n outD) =
+    Tick.cost (selection_sortD' xs outD).
+Proof.
+  induction xs as [| x xs]; simpl; intros.
+  - destruct n, outD; simpl; lia.
+  - destruct n, outD; simpl; try lia.
+    destruct (select x xs) eqn:Hselect.
+    destruct x2; simpl.
+    + admit.      
+    + pose proof (selectD_selectD'_eq x xs (exact l)) as Hdd'.
+      rewrite Hselect in Hdd'. specialize (Hdd' (exact n0) bottom).
+      assert (selectD x xs (pairA (exact n0) bottom) = selectD' x xs (exact l)).
+      { apply Hdd'; solve_approx. }
+      unfold AO_Exact in H0. simpl in H0.
+      rewrite H0. reflexivity.
+Admitted.    
+
+(** TODO: Finish this. *)
+
+(*
+Lemma selection_sortD_cost (xs : list nat) (outD : listA nat) :
+  Tick.cost (selection_sortD xs outD) <= (sizeX' 1 outD) * (length xs + 2).
+Proof.
+  intros. generalize dependent xs. induction outD;
+  intro; destruct xs; simpl; try rewrite IHoutD; try lia.
+  - pose proof (selectD_selectD'_leq n xs (exact (n :: xs))) as Hle.
+    unfold selectD' in Hle. simpl in Hle. lia.
+  - pose proof (selectD_selectD'_leq n xs (exact (n :: xs))) as Hle.
+    unfold selectD' in Hle. simpl in Hle. lia.
+Qed.
 
 Lemma head_selection_sortD_cost (xs : list nat) (outD : nat) :
   outD `is_approx` head_def (selection_sort xs (length xs)) 0 ->
@@ -148,17 +240,6 @@ Definition take_selection_sortD (n : nat) (xs : list nat) (outD : listA nat) :
   let+ list_takeD := takeD n (selection_sort xs (length xs)) outD in
   let+ xsD := thunkD (selection_sortD xs) list_takeD in
   Tick.ret xsD.
-
-Lemma selection_sortD_cost (xs : list nat) (outD : listA nat) :
-  Tick.cost (selection_sortD xs outD) <= (sizeX' 1 outD) * (length xs + 2).
-Proof.
-  intros. generalize dependent xs. induction outD;
-  intro; destruct xs; simpl; try rewrite IHoutD; try lia.
-  - pose proof (selectD_selectD'_leq n xs (exact (n :: xs))) as Hle.
-    unfold selectD' in Hle. simpl in Hle. lia.
-  - pose proof (selectD_selectD'_leq n xs (exact (n :: xs))) as Hle.
-    unfold selectD' in Hle. simpl in Hle. lia.
-Qed.
 
 Lemma headD_demand {a} (xs : list a) (d : a) (outD : a) : 
   sizeX 1 (Tick.val (headD xs d outD)) = 1.
@@ -196,7 +277,7 @@ Proof.
     rewrite selection_sortD_cost. rewrite H. rewrite takeD_demand. lia.
   - simpl. lia.
 Qed.
-
+*)
 
 (* I'm not sure if we need these... *)
 
